compiler/backend/passes/proofs/state_names_1ProofScript.sml
@@ -174,8 +174,17 @@ Definition rec_env_def:
     MAP (λ(fn,_). (fn,Recclosure f env fn)) f ++ env
 End
 
+Definition store_rel_def:
+  store_rel (Array vs1) (Array vs2) = LIST_REL v_rel vs1 vs2 ∧
+  store_rel _ _ = F
+End
+
+Definition state_rel_def:
+  state_rel st1 st2 = LIST_REL store_rel st1 st2
+End
+
 Inductive snext_res_rel:
-  (OPTREL (LIST_REL (LIST_REL v_rel)) ts ss ∧ cont_rel tk sk ⇒
+  (OPTREL state_rel ts ss ∧ cont_rel tk sk ⇒
    snext_res_rel (Act x tk ts) (Act x sk ss)) ∧
   (snext_res_rel Ret Ret) ∧
   (snext_res_rel Div Div) ∧
@@ -265,12 +274,12 @@ QED
 
 Theorem application_thm:
   application op tvs ts tk = (tr1,ts1,tk1) ∧
-  OPTREL (LIST_REL (LIST_REL v_rel)) ts ss ∧ cont_rel tk sk ∧
+  OPTREL state_rel ts ss ∧ cont_rel tk sk ∧
   LIST_REL v_rel tvs svs ∧
   num_args_ok op (LENGTH svs) ⇒
   ∃sr1 ss1 sk1.
     application op svs ss sk = (sr1,ss1,sk1) ∧
-    cont_rel tk1 sk1 ∧ OPTREL (LIST_REL (LIST_REL v_rel)) ts1 ss1 ∧
+    cont_rel tk1 sk1 ∧ OPTREL state_rel ts1 ss1 ∧
     step_res_rel tr1 sr1
 Proof
   Cases_on ‘op’ \\ fs [num_args_ok_def,LENGTH_EQ_NUM_compute,PULL_EXISTS]
@@ -349,16 +358,18 @@ Proof
     \\ simp [Once v_rel_cases] \\ strip_tac \\ gvs []
     \\ gvs [AllCaseEqs()]
     \\ Cases_on ‘ss’ \\ gvs []
+    \\ fs [state_rel_def]
     \\ imp_res_tac LIST_REL_LENGTH \\ fs []
     \\ simp [Once v_rel_cases]
-    \\ fs [LIST_REL_SNOC]
+    \\ fs [LIST_REL_SNOC,store_rel_def]
     \\ simp [LIST_REL_EL_EQN,EL_REPLICATE])
   >~ [‘Ref’] >-
    (gvs [application_def,step,step_res_rel_cases]
     \\ Cases_on ‘ts’ \\ Cases_on ‘ss’ \\ gvs []
+    \\ fs [state_rel_def]
     \\ imp_res_tac LIST_REL_LENGTH \\ fs []
     \\ simp [Once v_rel_cases]
-    \\ fs [LIST_REL_SNOC])
+    \\ fs [LIST_REL_SNOC,store_rel_def])
   >~ [‘Length’] >-
    (gvs [application_def,step,step_res_rel_cases]
     \\ qpat_x_assum ‘v_rel x h’ mp_tac
@@ -367,8 +378,12 @@ Proof
     \\ Cases_on ‘ts’ \\ Cases_on ‘ss’ \\ gvs []
     \\ imp_res_tac LIST_REL_LENGTH \\ fs [oEL_THM]
     \\ IF_CASES_TAC \\ gvs []
+    \\ gvs [LIST_REL_EL_EQN,state_rel_def]
+    \\ Cases_on `EL n x` \\ Cases_on `EL n x'` \\ gvs [store_rel_def]
+    \\ res_tac \\ Cases_on `EL n x` \\ gvs [store_rel_def]
     \\ simp [Once v_rel_cases]
-    \\ gvs [LIST_REL_EL_EQN])
+    \\ gvs [LIST_REL_EL_EQN,state_rel_def]
+    \\ imp_res_tac LIST_REL_LENGTH \\ fs [])
   >~ [‘Sub’] >-
    (gvs [application_def,step,step_res_rel_cases]
     \\ qpat_x_assum ‘v_rel x h’ mp_tac
@@ -380,10 +395,20 @@ Proof
     \\ Cases_on ‘ts’ \\ Cases_on ‘ss’ \\ gvs []
     \\ imp_res_tac LIST_REL_LENGTH \\ fs [oEL_THM]
     \\ rpt (IF_CASES_TAC \\ gvs [])
+    \\ gvs [state_rel_def]
+    \\ imp_res_tac LIST_REL_LENGTH \\ gvs [state_rel_def]
+    \\ Cases_on `EL n x` \\ Cases_on `EL n x'` \\ gvs [LIST_REL_EL_EQN]
+    \\ res_tac \\ Cases_on `EL n x` \\ gvs [store_rel_def]
+    \\ imp_res_tac LIST_REL_LENGTH \\ fs []
     \\ gvs [LIST_REL_EL_EQN]
-    \\ ntac 2 (simp [Once compile_rel_cases,env_rel_def])
-    \\ imp_res_tac integerTheory.NUM_POSINT_EXISTS \\ gvs []
-    \\ simp[Once v_rel_cases])
+    \\ Cases_on `0 ≤ i` \\ gvs []
+    >-
+      (imp_res_tac integerTheory.NUM_POSINT_EXISTS
+       \\ first_x_assum $ qspec_then `&n'` assume_tac
+       \\ gvs []
+       \\ Cases_on `n' < LENGTH l'` \\ gvs []
+       \\ gvs [Once v_rel_cases,LIST_REL_EL_EQN,state_rel_def])
+    >- simp [Once v_rel_cases,LIST_REL_EL_EQN,state_rel_def])
   >~ [‘UnsafeSub’] >-
    (gvs [application_def,step,step_res_rel_cases]
     \\ qpat_x_assum ‘v_rel x h’ mp_tac
@@ -395,9 +420,20 @@ Proof
     \\ Cases_on ‘ts’ \\ Cases_on ‘ss’ \\ gvs []
     \\ imp_res_tac LIST_REL_LENGTH \\ fs [oEL_THM]
     \\ rpt (IF_CASES_TAC \\ gvs [])
+    \\ gvs [state_rel_def]
+    \\ imp_res_tac LIST_REL_LENGTH \\ gvs [state_rel_def]
+    \\ Cases_on `EL n x` \\ Cases_on `EL n x'` \\ gvs [LIST_REL_EL_EQN]
+    \\ res_tac \\ Cases_on `EL n x` \\ gvs [store_rel_def]
+    \\ imp_res_tac LIST_REL_LENGTH \\ fs []
     \\ gvs [LIST_REL_EL_EQN]
-    \\ ntac 2 (simp [Once compile_rel_cases,env_rel_def])
-    \\ imp_res_tac integerTheory.NUM_POSINT_EXISTS \\ gvs [])
+    \\ Cases_on `0 ≤ i` \\ gvs []
+    >-
+      (imp_res_tac integerTheory.NUM_POSINT_EXISTS
+       \\ first_x_assum $ qspec_then `&n'` assume_tac
+       \\ gvs []
+       \\ Cases_on `n' < LENGTH l'` \\ gvs []
+       \\ gvs [Once v_rel_cases,LIST_REL_EL_EQN,state_rel_def])
+    >- simp [Once v_rel_cases,LIST_REL_EL_EQN,state_rel_def])
   >~ [‘Update’] >-
    (gvs [application_def,step,step_res_rel_cases]
     \\ qpat_x_assum ‘v_rel x h’ mp_tac
@@ -409,12 +445,27 @@ Proof
     \\ Cases_on ‘ts’ \\ Cases_on ‘ss’ \\ gvs []
     \\ imp_res_tac LIST_REL_LENGTH \\ fs [oEL_THM]
     \\ rpt (IF_CASES_TAC \\ gvs [])
+    \\ gvs [state_rel_def]
+    \\ imp_res_tac LIST_REL_LENGTH \\ gvs [state_rel_def]
+    \\ Cases_on `EL n x` \\ Cases_on `EL n x'` \\ gvs [LIST_REL_EL_EQN]
+    \\ res_tac \\ Cases_on `EL n x` \\ gvs [store_rel_def]
+    \\ imp_res_tac LIST_REL_LENGTH \\ fs []
     \\ gvs [LIST_REL_EL_EQN]
-    \\ ntac 2 (simp [Once compile_rel_cases,env_rel_def])
-    \\ imp_res_tac integerTheory.NUM_POSINT_EXISTS \\ gvs []
-    \\ gvs [EL_LUPDATE] \\ rw []
-    \\ gvs [EL_LUPDATE] \\ rw []
-    \\ simp [Once v_rel_cases] \\ strip_tac \\ gvs [])
+    \\ Cases_on `0 ≤ i` \\ gvs []
+    >-
+      (imp_res_tac integerTheory.NUM_POSINT_EXISTS
+       \\ first_x_assum $ qspec_then `&n'` assume_tac \\ gvs []
+       \\ Cases_on `n' < LENGTH l'` \\ gvs []
+       \\ simp [Once v_rel_cases,LIST_REL_EL_EQN,state_rel_def]
+       \\ rpt strip_tac
+       \\ gvs [EL_LUPDATE]
+       \\ Cases_on `n'' = n` \\ gvs []
+       \\ rw [LIST_REL_EL_EQN,store_rel_def]
+       \\ gvs [EL_LUPDATE]
+       \\ Cases_on `n'' = n'` \\ gvs []
+       \\ res_tac \\ Cases_on `EL n x` \\ gvs [store_rel_def]
+       \\ gvs [LIST_REL_EL_EQN])
+    >- simp [Once v_rel_cases,LIST_REL_EL_EQN,state_rel_def])
   >~ [‘UnsafeUpdate’] >-
    (gvs [application_def,step,step_res_rel_cases]
     \\ qpat_x_assum ‘v_rel x h’ mp_tac
@@ -426,12 +477,27 @@ Proof
     \\ Cases_on ‘ts’ \\ Cases_on ‘ss’ \\ gvs []
     \\ imp_res_tac LIST_REL_LENGTH \\ fs [oEL_THM]
     \\ rpt (IF_CASES_TAC \\ gvs [])
+    \\ gvs [state_rel_def]
+    \\ imp_res_tac LIST_REL_LENGTH \\ gvs [state_rel_def]
+    \\ Cases_on `EL n x` \\ Cases_on `EL n x'` \\ gvs [LIST_REL_EL_EQN]
+    \\ res_tac \\ Cases_on `EL n x` \\ gvs [store_rel_def]
+    \\ imp_res_tac LIST_REL_LENGTH \\ fs []
     \\ gvs [LIST_REL_EL_EQN]
-    \\ ntac 2 (simp [Once compile_rel_cases,env_rel_def])
-    \\ imp_res_tac integerTheory.NUM_POSINT_EXISTS \\ gvs []
-    \\ gvs [EL_LUPDATE] \\ rw []
-    \\ gvs [EL_LUPDATE] \\ rw []
-    \\ simp [Once v_rel_cases] \\ strip_tac \\ gvs [])
+    \\ Cases_on `0 ≤ i` \\ gvs []
+    >-
+      (imp_res_tac integerTheory.NUM_POSINT_EXISTS
+       \\ first_x_assum $ qspec_then `&n'` assume_tac \\ gvs []
+       \\ Cases_on `n' < LENGTH l'` \\ gvs []
+       \\ simp [Once v_rel_cases,LIST_REL_EL_EQN,state_rel_def]
+       \\ rpt strip_tac
+       \\ gvs [EL_LUPDATE]
+       \\ Cases_on `n'' = n` \\ gvs []
+       \\ rw [LIST_REL_EL_EQN,store_rel_def]
+       \\ gvs [EL_LUPDATE]
+       \\ Cases_on `n'' = n'` \\ gvs []
+       \\ res_tac \\ Cases_on `EL n x` \\ gvs [store_rel_def]
+       \\ gvs [LIST_REL_EL_EQN])
+    >- simp [Once v_rel_cases,LIST_REL_EL_EQN,state_rel_def])
   >~ [‘FFI’] >-
    (gvs [application_def,step,step_res_rel_cases]
     \\ qpat_x_assum ‘v_rel x h’ mp_tac
@@ -489,11 +555,11 @@ QED
 Theorem step_1_forward:
   ∀tr ts tk tr1 ts1 tk1 ss sr sk.
     step_n 1 (tr,ts,tk) = (tr1,ts1,tk1) ∧
-    cont_rel tk sk ∧ OPTREL (LIST_REL (LIST_REL v_rel)) ts ss ∧
+    cont_rel tk sk ∧ OPTREL state_rel ts ss ∧
     step_res_rel tr sr ∧ tr1 ≠ Error ⇒
     ∃m sr1 ss1 sk1.
       step_n (m+1) (sr,ss,sk) = (sr1,ss1,sk1) ∧
-      cont_rel tk1 sk1 ∧ OPTREL (LIST_REL (LIST_REL v_rel)) ts1 ss1 ∧
+      cont_rel tk1 sk1 ∧ OPTREL state_rel ts1 ss1 ∧
       step_res_rel tr1 sr1
 Proof
   rpt strip_tac
@@ -656,11 +722,11 @@ QED
 Theorem step_n_forward:
   ∀n tr ts tk tr1 ts1 tk1 ss sr sk.
     step_n n (tr,ts,tk) = (tr1,ts1,tk1) ∧
-    cont_rel tk sk ∧ OPTREL (LIST_REL (LIST_REL v_rel)) ts ss ∧
+    cont_rel tk sk ∧ OPTREL state_rel ts ss ∧
     step_res_rel tr sr ∧ tr1 ≠ Error ⇒
     ∃m sr1 ss1 sk1.
       step_n (m+n) (sr,ss,sk) = (sr1,ss1,sk1) ∧
-      cont_rel tk1 sk1 ∧ OPTREL (LIST_REL (LIST_REL v_rel)) ts1 ss1 ∧
+      cont_rel tk1 sk1 ∧ OPTREL state_rel ts1 ss1 ∧
       step_res_rel tr1 sr1
 Proof
   Induct \\ fs [] \\ rw []
@@ -682,7 +748,7 @@ QED
 
 Theorem step_until_halt_thm:
   step_res_rel tr sr ∧
-  OPTREL (LIST_REL (LIST_REL v_rel)) ts ss ∧
+  OPTREL state_rel ts ss ∧
   cont_rel tk sk ∧
   step_until_halt (tr,ts,tk) ≠ Err ⇒
   snext_res_rel (step_until_halt (tr,ts,tk))
@@ -720,7 +786,7 @@ QED
 
 Theorem semantics_thm:
   compile_rel e1 e2 ∧
-  OPTREL (LIST_REL (LIST_REL v_rel)) ts ss ∧
+  OPTREL state_rel ts ss ∧
   env_rel (freevars e1) tenv senv ∧
   cont_rel tk sk ⇒
   semantics e1 tenv ts tk --->
@@ -730,7 +796,7 @@ Proof
     ∀t1 t2.
       (∃e1 e2 ts ss tenv senv tk sk.
         compile_rel e1 e2 ∧
-        OPTREL (LIST_REL (LIST_REL v_rel)) ts ss ∧
+        OPTREL state_rel ts ss ∧
         env_rel (freevars e1) tenv senv ∧
         cont_rel tk sk ∧
         t1 = semantics e1 tenv ts tk ∧
@@ -789,7 +855,7 @@ Proof
   fs [stateLangTheory.itree_of_def] \\ rw []
   \\ irule semantics_thm
   \\ simp [Once cont_rel_cases]
-  \\ fs [env_rel_def]
+  \\ fs [env_rel_def,state_rel_def]
 QED
 
 val _ = export_theory ();
